Foundation/Modal/Kripke/Hilbert/KD.lean
@@ -8,42 +8,32 @@ open Geachean
 
 namespace Kripke.FrameClass
 
-protected abbrev serial : FrameClass := { F | Serial F }
-
-namespace serial
-
-lemma isMultiGeachean : FrameClass.serial = FrameClass.multiGeachean {⟨0, 0, 1, 1⟩} := by
-  ext F;
-  simp [Geachean.serial_def, MultiGeachean]
-
-@[simp]
-lemma nonempty : FrameClass.serial.Nonempty := by simp [isMultiGeachean]
-
-lemma validates_AxiomD : FrameClass.serial.ValidatesFormula (Axioms.D (.atom 0)) := by
-  rintro F F_serial _ rfl;
-  apply validate_AxiomD_of_serial $ by assumption
-
-lemma validates_HilbertKD : FrameClass.serial.Validates Hilbert.KD.axioms := by
-  apply FrameClass.Validates.withAxiomK;
-  apply validates_AxiomD;
-
-end serial
+protected abbrev serial : FrameClass := { F | IsSerial _ F.Rel }
 
 end Kripke.FrameClass
 
 
-namespace Hilbert.KD
+namespace Hilbert.KD.Kripke
 
-instance Kripke.sound : Sound (Hilbert.KD) Kripke.FrameClass.serial :=
-  instSound_of_validates_axioms FrameClass.serial.validates_HilbertKD
+instance sound : Sound (Hilbert.KD) Kripke.FrameClass.serial :=
+  instSound_of_validates_axioms $ by
+    apply FrameClass.Validates.withAxiomK;
+    rintro F F_serial φ rfl;
+    apply validate_AxiomD_of_serial (ser := F_serial);
 
-instance Kripke.consistent : Entailment.Consistent (Hilbert.KD) :=
-  consistent_of_sound_frameclass FrameClass.serial (by simp)
+instance consistent : Entailment.Consistent (Hilbert.KD) :=
+  consistent_of_sound_frameclass FrameClass.serial $ by
+    use whitepoint;
+    apply Set.mem_setOf_eq.mpr;
+    infer_instance;
 
-instance Kripke.canonical : Canonical (Hilbert.KD) Kripke.FrameClass.serial := ⟨Canonical.serial⟩
+instance canonical : Canonical (Hilbert.KD) Kripke.FrameClass.serial := ⟨by
+  apply Set.mem_setOf_eq.mpr;
+  infer_instance;
+⟩
 
-instance Kripke.complete : Complete (Hilbert.KD) Kripke.FrameClass.serial := inferInstance
+instance complete : Complete (Hilbert.KD) Kripke.FrameClass.serial := inferInstance
 
-end Hilbert.KD
+end Hilbert.KD.Kripke
 
 end LO.Modal
