Foundation/Modal/Kripke/Hilbert/KT.lean
@@ -6,36 +6,24 @@ open Kripke
 open Hilbert.Kripke
 open Geachean
 
-namespace Kripke
-
-variable {F : Frame}
-
-protected abbrev FrameClass.refl : FrameClass := { F | IsRefl _ F }
-
-namespace FrameClass.refl
-
-@[simp] lemma nonempty : FrameClass.refl.Nonempty := by use whitepoint; tauto;
-
-lemma validates_AxiomT : FrameClass.refl.ValidatesFormula (Axioms.T (.atom 0)) := by
-  apply ValidatesFormula_of;
-  apply Kripke.validate_AxiomT_of_reflexive;
-
-lemma validates_HilbertKT : FrameClass.refl.Validates Hilbert.KT.axioms := Validates.withAxiomK validates_AxiomT
-
-end FrameClass.refl
-
-end Kripke
-
+protected abbrev Kripke.FrameClass.refl : FrameClass := { F | IsRefl _ F }
 
 namespace Hilbert.KT
 
-instance Kripke.sound : Sound (Hilbert.KT) Kripke.FrameClass.refl :=
-  instSound_of_validates_axioms Kripke.FrameClass.refl.validates_HilbertKT
+instance Kripke.sound : Sound (Hilbert.KT) Kripke.FrameClass.refl := instSound_of_validates_axioms $ by
+  apply FrameClass.Validates.withAxiomK;
+  rintro F F_refl _ rfl;
+  exact Kripke.validate_AxiomT_of_reflexive (refl := F_refl);
 
-instance Kripke.consistent : Entailment.Consistent (Hilbert.KT) :=
-  consistent_of_sound_frameclass Kripke.FrameClass.refl (by simp)
+instance Kripke.consistent : Entailment.Consistent (Hilbert.KT) := consistent_of_sound_frameclass Kripke.FrameClass.refl $ by
+  use whitepoint;
+  apply Set.mem_setOf_eq.mpr;
+  infer_instance;
 
-instance Kripke.canonical : Canonical (Hilbert.KT) Kripke.FrameClass.refl := ⟨Canonical.reflexive⟩
+instance Kripke.canonical : Canonical (Hilbert.KT) Kripke.FrameClass.refl := ⟨by
+  apply Set.mem_setOf_eq.mpr;
+  infer_instance;
+⟩
 
 instance Kripke.complete : Complete (Hilbert.KT) Kripke.FrameClass.refl := inferInstance
 
