Foundation/Modal/Kripke/Hilbert/KB5.lean
@@ -6,40 +6,28 @@ open Kripke
 open Hilbert.Kripke
 open Geachean
 
-abbrev Kripke.FrameClass.symm_eucl : FrameClass := { F | Symmetric F ∧ Euclidean F }
+abbrev Kripke.FrameClass.symm_eucl : FrameClass := { F | IsSymm _ F ∧ IsEuclidean _ F }
 
-namespace Kripke.FrameClass.symm_eucl
+namespace Hilbert.KB5.Kripke
 
-lemma isMultiGeachean : FrameClass.symm_eucl = FrameClass.multiGeachean {⟨0, 1, 0, 1⟩, ⟨1, 1, 0, 1⟩} := by
-  ext F;
-  simp [Geachean.euclidean_def, Geachean.symmetric_def, MultiGeachean]
-
-@[simp]
-lemma nonempty : FrameClass.symm_eucl.Nonempty := by simp [isMultiGeachean]
-
-lemma validates_HilbertKB5 : Kripke.FrameClass.symm_eucl.Validates Hilbert.KB5.axioms := by
+instance sound : Sound (Hilbert.KB5) Kripke.FrameClass.symm_eucl := instSound_of_validates_axioms $ by
   apply FrameClass.Validates.withAxiomK;
-  rintro F ⟨F_symm, F_eucl⟩ φ (rfl | rfl);
-  . exact validate_AxiomB_of_symmetric $ by assumption;
-  . exact validate_AxiomFive_of_euclidean $ by assumption;
+  rintro F ⟨_, _⟩ _ (rfl | rfl);
+  . exact validate_AxiomB_of_symmetric;
+  . exact validate_AxiomFive_of_euclidean;
 
-end Kripke.FrameClass.symm_eucl
+instance consistent : Entailment.Consistent (Hilbert.KB5) := consistent_of_sound_frameclass Kripke.FrameClass.symm_eucl $ by
+  use whitepoint;
+  constructor <;> infer_instance;
 
+instance canonical : Canonical (Hilbert.KB5) Kripke.FrameClass.symm_eucl := ⟨by
+  apply Set.mem_setOf_eq.mpr;
+  constructor <;> infer_instance;
+⟩
 
-
-namespace Hilbert.KB5
-
-instance Kripke.sound : Sound (Hilbert.KB5) Kripke.FrameClass.symm_eucl :=
-  instSound_of_validates_axioms Kripke.FrameClass.symm_eucl.validates_HilbertKB5
-
-instance Kripke.consistent : Entailment.Consistent (Hilbert.KB5) :=
-  consistent_of_sound_frameclass Kripke.FrameClass.symm_eucl (by simp)
-
-instance Kripke.canonical : Canonical (Hilbert.KB5) Kripke.FrameClass.symm_eucl := ⟨⟨Canonical.symmetric, Canonical.euclidean⟩⟩
-
-instance Kripke.complete : Complete (Hilbert.KB5) Kripke.FrameClass.symm_eucl := inferInstance
+instance complete : Complete (Hilbert.KB5) Kripke.FrameClass.symm_eucl := inferInstance
 
 
-end Hilbert.KB5
+end Hilbert.KB5.Kripke
 
 end LO.Modal
