Foundation/Modal/Kripke/Hilbert/KDB.lean
@@ -6,39 +6,27 @@ open Kripke
 open Hilbert.Kripke
 open Geachean
 
-abbrev Kripke.FrameClass.serial_symm : FrameClass := { F | Serial F ∧ Symmetric F }
+abbrev Kripke.FrameClass.serial_symm : FrameClass := { F | IsSerial _ F ∧ IsSymm _ F }
 
-namespace Kripke.FrameClass.serial_symm
+namespace Hilbert.KDB.Kripke
 
-lemma isMultiGeachean : FrameClass.serial_symm = FrameClass.multiGeachean {⟨0, 0, 1, 1⟩, ⟨0, 1, 0, 1⟩} := by
-  ext F;
-  simp [Geachean.serial_def, Geachean.symmetric_def, MultiGeachean]
-
-@[simp]
-lemma nonempty : FrameClass.serial_symm.Nonempty := by simp [isMultiGeachean]
-
-lemma validates_HilbertKDB : Kripke.FrameClass.serial_symm.Validates Hilbert.KDB.axioms := by
+instance sound : Sound (Hilbert.KDB) Kripke.FrameClass.serial_symm := instSound_of_validates_axioms $ by
   apply FrameClass.Validates.withAxiomK;
-  rintro F ⟨F_serial, F_eucl⟩ φ (rfl | rfl);
-  . exact validate_AxiomD_of_serial $ by assumption;
-  . exact validate_AxiomB_of_symmetric $ by assumption;
+  rintro F ⟨_, _⟩ _ (rfl | rfl);
+  . exact validate_AxiomD_of_serial;
+  . exact validate_AxiomB_of_symmetric;
 
-end Kripke.FrameClass.serial_symm
+instance consistent : Entailment.Consistent (Hilbert.KDB) := consistent_of_sound_frameclass Kripke.FrameClass.serial_symm $ by
+  use whitepoint;
+  constructor <;> infer_instance;
 
+instance canonical : Canonical (Hilbert.KDB) Kripke.FrameClass.serial_symm := ⟨by
+  apply Set.mem_setOf_eq.mpr;
+  constructor <;> infer_instance;
+⟩
 
+instance complete : Complete (Hilbert.KDB) Kripke.FrameClass.serial_symm := inferInstance
 
-namespace Hilbert.KDB
-
-instance Kripke.sound : Sound (Hilbert.KDB) Kripke.FrameClass.serial_symm :=
-  instSound_of_validates_axioms Kripke.FrameClass.serial_symm.validates_HilbertKDB
-
-instance Kripke.consistent : Entailment.Consistent (Hilbert.KDB) :=
-  consistent_of_sound_frameclass Kripke.FrameClass.serial_symm (by simp)
-
-instance Kripke.canonical : Canonical (Hilbert.KDB) Kripke.FrameClass.serial_symm := ⟨⟨Canonical.serial, Canonical.symmetric⟩⟩
-
-instance Kripke.complete : Complete (Hilbert.KDB) Kripke.FrameClass.serial_symm := inferInstance
-
-end Hilbert.KDB
+end Hilbert.KDB.Kripke
 
 end LO.Modal
