Foundation/Modal/Kripke/Hilbert/KTB.lean
@@ -8,37 +8,27 @@ open Kripke
 open Hilbert.Kripke
 open Geachean
 
-abbrev Kripke.FrameClass.refl_symm : FrameClass := { F | Reflexive F ∧ Symmetric F }
+abbrev Kripke.FrameClass.refl_symm : FrameClass := { F | IsRefl _ F ∧ IsSymm _ F }
 
-abbrev Kripke.FrameClass.finite_refl_symm: FrameClass := { F | F.IsFinite ∧ Reflexive F.Rel ∧ Symmetric F.Rel }
-
-namespace Kripke.FrameClass.refl_symm
-
-lemma isMultiGeachean : FrameClass.refl_symm = FrameClass.multiGeachean {⟨0, 0, 1, 0⟩, ⟨0, 1, 0, 1⟩} := by
-  ext F;
-  simp [Geachean.reflexive_def, Geachean.symmetric_def, MultiGeachean]
-
-@[simp]
-lemma nonempty : FrameClass.refl_symm.Nonempty := by simp [isMultiGeachean]
-
-lemma validates_HilbertKTB : Kripke.FrameClass.refl_symm.Validates Hilbert.KTB.axioms := by
-  apply FrameClass.Validates.withAxiomK;
-  rintro F ⟨F_refl, F_symm⟩ φ (rfl | rfl);
-  . exact validate_AxiomT_of_reflexive $ by assumption;
-  . exact validate_AxiomB_of_symmetric $ by assumption;
-
-end Kripke.FrameClass.refl_symm
-
+abbrev Kripke.FrameClass.finite_refl_symm: FrameClass := { F | Finite F.World ∧ IsRefl _ F ∧ IsSymm _ F }
 
 namespace Hilbert.KTB.Kripke
 
-instance sound : Sound (Hilbert.KTB) Kripke.FrameClass.refl_symm :=
-  instSound_of_validates_axioms Kripke.FrameClass.refl_symm.validates_HilbertKTB
+instance sound : Sound (Hilbert.KTB) Kripke.FrameClass.refl_symm := instSound_of_validates_axioms $ by
+  apply FrameClass.Validates.withAxiomK;
+  rintro F ⟨_, _⟩ _ (rfl | rfl);
+  . exact validate_AxiomT_of_reflexive;
+  . exact validate_AxiomB_of_symmetric;
 
-instance consistent : Entailment.Consistent (Hilbert.KTB) :=
-  consistent_of_sound_frameclass Kripke.FrameClass.refl_symm (by simp)
+instance consistent : Entailment.Consistent (Hilbert.KTB) := consistent_of_sound_frameclass
+  Kripke.FrameClass.refl_symm $ by
+    use whitepoint;
+    constructor <;> infer_instance;
 
-instance canonical : Canonical (Hilbert.KTB) Kripke.FrameClass.refl_symm := ⟨⟨Canonical.reflexive, Canonical.symmetric⟩⟩
+instance canonical : Canonical (Hilbert.KTB) Kripke.FrameClass.refl_symm :=  ⟨by
+  apply Set.mem_setOf_eq.mpr;
+  constructor <;> infer_instance;
+⟩
 
 instance complete : Complete (Hilbert.KTB) Kripke.FrameClass.refl_symm := inferInstance
 
