Foundation/Modal/Kripke/Hilbert/S4.lean
@@ -7,36 +7,32 @@ open Kripke
 open Hilbert.Kripke
 open Geachean
 
-abbrev Kripke.FrameClass.preorder : FrameClass := { F | Reflexive F ∧ Transitive F }
-abbrev Kripke.FrameClass.finite_preorder: FrameClass := { F | F.IsFinite ∧ Reflexive F.Rel ∧ Transitive F.Rel }
 
-namespace Kripke.FrameClass.preorder
+namespace Kripke
 
-lemma isMultiGeachean : FrameClass.preorder = FrameClass.multiGeachean {⟨0, 0, 1, 0⟩, ⟨0, 2, 1, 0⟩} := by
-  ext F;
-  simp [Geachean.reflexive_def, Geachean.transitive_def, MultiGeachean]
+protected abbrev FrameClass.preorder : FrameClass := { F | IsPreorder _ F }
 
-@[simp]
-lemma nonempty : FrameClass.preorder.Nonempty := by simp [isMultiGeachean]
+protected abbrev FrameClass.finite_preorder: FrameClass := { F | Finite F.World ∧ IsPreorder _ F.Rel }
 
-lemma validates_HilbertS4 : Kripke.FrameClass.preorder.Validates Hilbert.S4.axioms := by
-  apply FrameClass.Validates.withAxiomK;
-  rintro F ⟨F_refl, F_trans⟩ φ (rfl | rfl);
-  . exact validate_AxiomT_of_reflexive F_refl;
-  . exact validate_AxiomFour_of_transitive F_trans;
-
-end Kripke.FrameClass.preorder
+end Kripke
 
 
 namespace Hilbert.S4.Kripke
 
-instance sound : Sound (Hilbert.S4) Kripke.FrameClass.preorder :=
-  instSound_of_validates_axioms Kripke.FrameClass.preorder.validates_HilbertS4
+instance sound : Sound (Hilbert.S4) Kripke.FrameClass.preorder := instSound_of_validates_axioms $ by
+  apply FrameClass.Validates.withAxiomK;
+  rintro F ⟨_, _⟩ _ (rfl | rfl);
+  . exact validate_AxiomT_of_reflexive;
+  . exact validate_AxiomFour_of_transitive;
 
-instance consistent : Entailment.Consistent (Hilbert.S4) :=
-  consistent_of_sound_frameclass Kripke.FrameClass.preorder (by simp)
+instance consistent : Entailment.Consistent (Hilbert.S4) := consistent_of_sound_frameclass Kripke.FrameClass.preorder $ by
+  use whitepoint;
+  constructor;
 
-instance canonical : Canonical (Hilbert.S4) Kripke.FrameClass.preorder := ⟨⟨Canonical.reflexive, Canonical.transitive⟩⟩
+instance canonical : Canonical (Hilbert.S4) Kripke.FrameClass.preorder := ⟨by
+  apply Set.mem_setOf_eq.mpr;
+  constructor;
+⟩
 
 instance complete : Complete (Hilbert.S4) Kripke.FrameClass.preorder := inferInstance
 
@@ -44,17 +40,14 @@ open finestFilterationTransitiveClosureModel in
 instance finiteComplete : Complete (Hilbert.S4) Kripke.FrameClass.finite_preorder := ⟨by
   intro φ hp;
   apply Kripke.complete.complete;
-  intro F ⟨F_refl, F_trans⟩ V x;
+  rintro F ⟨F_refl, F_trans⟩ V x;
   let M : Kripke.Model := ⟨F, V⟩;
   let FM := finestFilterationTransitiveClosureModel M φ.subformulas;
-  apply filteration FM (finestFilterationTransitiveClosureModel.filterOf F_trans) (by aesop) |>.mpr;
+  apply filteration FM (finestFilterationTransitiveClosureModel.filterOf) (by aesop) |>.mpr;
   apply hp;
-  refine ⟨?_, ?_, ?_⟩;
-  . apply Frame.isFinite_iff _ |>.mpr
-    apply FilterEqvQuotient.finite;
+  refine ⟨?_, by sorry⟩;
+  . apply FilterEqvQuotient.finite;
     simp;
-  . exact reflexive_of_transitive_reflexive F_trans F_refl;
-  . exact finestFilterationTransitiveClosureModel.transitive;
 ⟩
 
 end Hilbert.S4.Kripke
