Foundation/Modal/Kripke/Hilbert/S4Point2.lean
@@ -8,37 +8,29 @@ open Kripke
 open Hilbert.Kripke
 open Geachean
 
-abbrev Kripke.FrameClass.confluent_preorder : FrameClass := { F | Reflexive F ∧ Transitive F ∧ Confluent F  }
-abbrev Kripke.FrameClass.finite_confluent_preorder : FrameClass := { F | F.IsFinite ∧ Reflexive F ∧ Transitive F ∧ Confluent F  }
-
-namespace Kripke.FrameClass.confluent_preorder
-
-lemma isMultiGeachean : FrameClass.confluent_preorder = FrameClass.multiGeachean {⟨0, 0, 1, 0⟩, ⟨0, 2, 1, 0⟩, ⟨1, 1, 1, 1⟩} := by
-  ext F;
-  simp [Geachean.reflexive_def, Geachean.transitive_def, Geachean.confluent_def, MultiGeachean]
-
-@[simp]
-lemma nonempty : FrameClass.confluent_preorder.Nonempty := by simp [isMultiGeachean]
-
-lemma validates_HilbertS4Point2 : Kripke.FrameClass.confluent_preorder.Validates Hilbert.S4Point2.axioms := by
-  apply FrameClass.Validates.withAxiomK;
-  rintro F ⟨F_refl, F_trans, F_conn⟩ φ (rfl | rfl | rfl);
-  . exact validate_AxiomT_of_reflexive F_refl;
-  . exact validate_AxiomFour_of_transitive F_trans;
-  . exact validate_AxiomPoint2_of_confluent F_conn;
-
-end Kripke.FrameClass.confluent_preorder
-
+abbrev Kripke.FrameClass.confluent_preorder : FrameClass := { F | IsPreorder _ F ∧ IsConfluent _ F  }
+abbrev Kripke.FrameClass.finite_confluent_preorder : FrameClass := { F | Finite F.World ∧ IsPreorder _ F ∧ IsConfluent _ F }
 
 namespace Hilbert.S4Point2.Kripke
 
-instance sound : Sound (Hilbert.S4Point2) Kripke.FrameClass.confluent_preorder :=
-  instSound_of_validates_axioms FrameClass.confluent_preorder.validates_HilbertS4Point2
+instance sound : Sound (Hilbert.S4Point2) Kripke.FrameClass.confluent_preorder := instSound_of_validates_axioms $ by
+  apply FrameClass.Validates.withAxiomK;
+  rintro F ⟨_, _⟩ _ (rfl | rfl | rfl);
+  . exact validate_AxiomT_of_reflexive;
+  . exact validate_AxiomFour_of_transitive;
+  . exact validate_AxiomPoint2_of_confluent;
 
 instance consistent : Entailment.Consistent (Hilbert.S4Point2) :=
-  consistent_of_sound_frameclass FrameClass.confluent_preorder (by simp)
+  consistent_of_sound_frameclass FrameClass.confluent_preorder $ by
+    use whitepoint;
+    refine ⟨inferInstance, inferInstance⟩;
 
-instance canonical : Canonical (Hilbert.S4Point2) Kripke.FrameClass.confluent_preorder := ⟨⟨Canonical.reflexive, Canonical.transitive, Canonical.confluent⟩⟩
+instance canonical : Canonical (Hilbert.S4Point2) Kripke.FrameClass.confluent_preorder := ⟨by
+  apply Set.mem_setOf_eq.mpr;
+  refine ⟨?_, ?_⟩;
+  . constructor;
+  . infer_instance;
+⟩
 
 instance complete : Complete (Hilbert.S4Point2) Kripke.FrameClass.confluent_preorder := inferInstance
 
@@ -52,16 +44,16 @@ open
 instance finite_complete : Complete (Hilbert.S4Point2) Kripke.FrameClass.finite_confluent_preorder := ⟨by
   intro φ hφ;
   apply Kripke.complete.complete;
-  rintro F ⟨F_refl, F_trans, F_con⟩ V r;
+  rintro F ⟨_, _⟩ V r;
   let M : Kripke.Model := ⟨F, V⟩;
   let RM := M↾r;
-  have RM_refl : Reflexive RM.Rel := Frame.pointGenerate.rel_refl F_refl;
-  have RM_trans : Transitive RM.Rel := Frame.pointGenerate.rel_trans F_trans;
+  -- have RM_refl : Reflexive RM.Rel := Frame.pointGenerate.rel_refl F_refl;
+  -- have RM_trans : IsTrans _ RM.Rel := inferInstance;
 
   apply Model.pointGenerate.modal_equivalent_at_root (M := M) (r := r) |>.mp;
 
-  let FRM := finestFilterationTransitiveClosureModel RM (φ.subformulas);
-  apply filteration FRM (finestFilterationTransitiveClosureModel.filterOf RM_trans) (by aesop) |>.mpr;
+  let FRM := finestFilterationTransitiveClosureModel (M↾r) (φ.subformulas);
+  apply filteration FRM (finestFilterationTransitiveClosureModel.filterOf) (by aesop) |>.mpr;
   apply hφ;
 
   refine ⟨?_, ?_, ?_, ?_⟩;
