Foundation/Modal/Kripke/Hilbert/Triv.lean
@@ -7,27 +7,10 @@ open Kripke
 open Hilbert.Kripke
 open Geachean
 
-protected abbrev Kripke.FrameClass.refl_corefl : FrameClass := { F | Reflexive F ∧ Coreflexive F }
-protected abbrev Kripke.FrameClass.equality : FrameClass := { F | Equality F }
+protected abbrev Kripke.FrameClass.refl_corefl : FrameClass := { F | IsRefl _ F ∧ IsCoreflexive _ F }
+protected abbrev Kripke.FrameClass.equality : FrameClass := { F | IsEquality _ F }
 
-namespace Kripke.FrameClass.refl_corefl
-
-lemma isMultiGeachean : FrameClass.refl_corefl = FrameClass.multiGeachean {⟨0, 0, 1, 0⟩, ⟨0, 1, 0, 0⟩} := by
-  ext F;
-  simp [Geachean.reflexive_def, Geachean.coreflexive_def, MultiGeachean]
-
-@[simp]
-lemma nonempty : FrameClass.refl_corefl.Nonempty := by simp [isMultiGeachean]
-
-lemma validates_HilbertTriv : Kripke.FrameClass.refl_corefl.Validates Hilbert.Triv.axioms := by
-  apply FrameClass.Validates.withAxiomK;
-  rintro F ⟨F_refl, F_trans⟩ φ (rfl | rfl);
-  . apply FrameClass.refl.validates_AxiomT; repeat tauto;
-  . apply FrameClass.corefl.validates_AxiomTc; repeat tauto;
-
-end Kripke.FrameClass.refl_corefl
-
-
+/-
 lemma Kripke.FrameClass.eq_equality_refl_corefl : Kripke.FrameClass.equality = Kripke.FrameClass.refl_corefl := by
   ext F;
   constructor;
@@ -37,29 +20,41 @@ lemma Kripke.FrameClass.eq_equality_refl_corefl : Kripke.FrameClass.equality = K
     . exact corefl_of_equality hEq;
   . rintro ⟨hRefl, hCorefl⟩;
     exact equality_of_refl_corefl hRefl hCorefl;
+-/
 
+namespace Hilbert.Triv.Kripke
 
-namespace Hilbert.Triv
+instance sound_refl_corefl : Sound (Hilbert.Triv) Kripke.FrameClass.refl_corefl :=
+  instSound_of_validates_axioms $ by
+    apply FrameClass.Validates.withAxiomK;
+    rintro F ⟨_, _⟩ _ (rfl | rfl);
+    . exact validate_AxiomT_of_reflexive;
+    . exact validate_AxiomTc_of_coreflexive;
 
-instance Kripke.sound_refl_corefl : Sound (Hilbert.Triv) Kripke.FrameClass.refl_corefl :=
-  instSound_of_validates_axioms Kripke.FrameClass.refl_corefl.validates_HilbertTriv
-
-instance Kripke.sound_equality : Sound (Hilbert.Triv) Kripke.FrameClass.equality := by
+/-
+instance sound_equality : Sound (Hilbert.Triv) Kripke.FrameClass.equality := by
   rw [Kripke.FrameClass.eq_equality_refl_corefl];
   exact Kripke.sound_refl_corefl;
+-/
 
-instance Kripke.consistent : Entailment.Consistent (Hilbert.Triv) :=
-  consistent_of_sound_frameclass Kripke.FrameClass.refl_corefl (by simp)
+instance consistent : Entailment.Consistent (Hilbert.Triv) := consistent_of_sound_frameclass Kripke.FrameClass.refl_corefl $ by
+  use whitepoint;
+  constructor <;> infer_instance;
 
-instance Kripke.cannonical_refl_corefl : Canonical (Hilbert.Triv) Kripke.FrameClass.refl_corefl := ⟨⟨Canonical.reflexive, Canonical.coreflexive⟩⟩
+instance cannonical_refl_corefl : Canonical (Hilbert.Triv) Kripke.FrameClass.refl_corefl := ⟨by
+  apply Set.mem_setOf_eq.mpr;
+  constructor <;> infer_instance;
+⟩
 
-instance Kripke.complete_refl_corefl : Complete (Hilbert.Triv) Kripke.FrameClass.refl_corefl := inferInstance
+instance complete_refl_corefl : Complete (Hilbert.Triv) Kripke.FrameClass.refl_corefl := inferInstance
 
-instance Kripke.complete_equality : Complete (Hilbert.Triv) Kripke.FrameClass.equality := by
+/-
+instance complete_equality : Complete (Hilbert.Triv) Kripke.FrameClass.equality := by
   rw [Kripke.FrameClass.eq_equality_refl_corefl];
   exact Kripke.complete_refl_corefl;
+-/
 
-end Hilbert.Triv
+end Hilbert.Triv.Kripke
 
 
 end LO.Modal
